SSA/Core/Framework/Macro.lean
@@ -188,10 +188,15 @@ def parseSignature (ref : TSyntax ``LeanMLIR.Parser.signature) : m Term :=
       | `(argumentList| ${$args})  => pure args
       | `(argumentList| ($args,*)) => `([$args,*])
       | ref => throwUnexpectedSyntax ref
+    mkReturnType (ret : Term) : m Term := do
+      -- TODO: for now we assume there is just a single return type
+      `([$ret])
+
     mkSignature (argumentTypes : TSyntax ``argumentList) (regions : Array Term)
         (returnType : Term) (effectKind : Term) :
         m Term := do
       let argumentTypes ← parseArgumentList argumentTypes
+      let returnType ← mkReturnType returnType
       `(_root_.Signature.mkEffectful $argumentTypes [$regions,*] $returnType $effectKind)
     parseFunction (regions : Array Term)
         (ref : TSyntax ``LeanMLIR.Parser.function) :
